add a bunch of code on transfer

implementation/InferLazy.hs
@@ -1,13 +1,15 @@
-{-# LANGUAGE LambdaCase, MultiWayIf #-}
+{-# LANGUAGE LambdaCase #-}
+{-# LANGUAGE MultiWayIf #-}
+
 module InferLazy where
 
 import Data.List
-
 import LazyDef
 import TestCase
+
 {- A lazy subtyping algorithm:
 
-A,B := a | ^a | Int | A -> B | forall a. A | 
+A,B := a | ^a | Int | A -> B | forall a. A |
 T ::= . | T,a | T, lbs <: ^a <: ubs |- A <: B
 
 Algorithm:
@@ -40,38 +42,38 @@ Algorithm:
 08. T |- A <: forall b . B             --> T,b |- A <: C                                          (rule 10)
 [0, -1, 0, -1] -> (-1, -1)
 
-09. T[lbs <: ^a < ubs] |- ^a <: A -> B --> T[^a1,^a2,lbs <: ^a < ubs ∪ {^a1->^a2}] |- ^a1 -> ^a2 <: A -> B  
-          when not monotype (A->B)  
+09. T[lbs <: ^a < ubs] |- ^a <: A -> B --> T[^a1,^a2,lbs <: ^a < ubs ∪ {^a1->^a2}] |- ^a1 -> ^a2 <: A -> B
+          when not monotype (A->B)
 [-1, 0, +2, +?] -> (-1, +?)
 
 09'. T[lbs <: ^a < ubs] |- ^a <: A -> B --> ([A->B/^a]_[] T) [lbs <: ^a < ubs ∪ {A->B}] |-
-          when monotype (A->B)  
+          when monotype (A->B)
 [0, 0, 0, -1] -> (0, -1)
 
-10. T[lbs <: ^a < ubs] |- A -> B <: ^a --> T[^a1,^a2, lbs ∪ {^a1,^a2} <: ^a < ubs] |- A -> B <: ^a1 -> ^a2   
-          when not monotype (A->B)  
+10. T[lbs <: ^a < ubs] |- A -> B <: ^a --> T[^a1,^a2, lbs ∪ {^a1,^a2} <: ^a < ubs] |- A -> B <: ^a1 -> ^a2
+          when not monotype (A->B)
 [-1, 0, +2, +?] -> (-1, +?)
 
-10'. T[lbs <: ^a < ubs] |- A -> B <: ^a --> ([A->B/^a]_[] T) [lbs ∪ {A->B} <: ^a < ubs] |- 
-          when monotype (A->B)  
+10'. T[lbs <: ^a < ubs] |- A -> B <: ^a --> ([A->B/^a]_[] T) [lbs ∪ {A->B} <: ^a < ubs] |-
+          when monotype (A->B)
 [0, 0, 0, -1] -> (0, -1)
 
-11. T[a][lbs <: ^b < ubs] |- a <: ^b   --> T[a][lbs ∪ {a} <: ^b < ubs] 
+11. T[a][lbs <: ^b < ubs] |- a <: ^b   --> T[a][lbs ∪ {a} <: ^b < ubs]
 [0, 0, 0, -1] -> (0, -1)
 
-12. T[a][lbs <: ^b < ubs] |- ^b <: a   --> T[a][lbs <: ^b <: ubs ∪ {a}] 
+12. T[a][lbs <: ^b < ubs] |- ^b <: a   --> T[a][lbs <: ^b <: ubs ∪ {a}]
 [0, 0, 0, -1] -> (0, -1)
 
-13. T[lbs <: ^b < ubs] |- Int <: ^b    --> T[a][lbs U {Int} <: ^b <: ubs] 
+13. T[lbs <: ^b < ubs] |- Int <: ^b    --> T[a][lbs U {Int} <: ^b <: ubs]
 [0, 0, 0, -1] -> (0, -1)
 
-14. T[lbs <: ^b < ubs] |- ^b <: Int    --> T[a][lbs <: ^b <: ubs ∪ {Int}] 
+14. T[lbs <: ^b < ubs] |- ^b <: Int    --> T[a][lbs <: ^b <: ubs ∪ {Int}]
 [0, 0, 0, -1] -> (0, -1)
 
-15. T[^a][lbs <: ^b < ubs] |- ^a <: ^b --> T[^a][lbs ∪ {^a} <: ^b < ubs] 
+15. T[^a][lbs <: ^b < ubs] |- ^a <: ^b --> T[^a][lbs ∪ {^a} <: ^b < ubs]
 [0, 0, 0, -1] -> (0, -1)
 
-16. T[^a][lbs <: ^b < ubs] |- ^b <: ^a --> T[^a][lbs <: ^b < ubs ∪ {^a}] 
+16. T[^a][lbs <: ^b < ubs] |- ^b <: ^a --> T[^a][lbs <: ^b < ubs ∪ {^a}]
 [0, 0, 0, -1] -> (0, -1)
 
 --------------
@@ -81,23 +83,22 @@ Algorithm:
 [A/^a]_E (T,L <: ^a <: R)   = T, reverse E, L <: ^a <: R                 ^a notin fv(A) and ^a notin fv(E)
 [A/^a]_E (T,L <: ^b <: R)   = [A/^a]_E T, L <: ^b <: R          ^b notin FV(A + E)
 [A/^a]_E (T, L <: ^b <: R)  = [A/^a]_{E, L <: ^b <: R} T        (^b in FV(A) or ^b in FV(E)) and ^a notin(L+R)
-[A/^a]_E (T, a)             = [A/^a]_{E} T, a                   a notin FV(A+ E) 
+[A/^a]_E (T, a)             = [A/^a]_{E} T, a                   a notin FV(A+ E)
 [A/^a]_E (T |- B <: C)      = [A/^a]_(E, B <: C) T             fv(B + C) ∩ fv(A + E) != Φ
 [A/^a]_E (T |- B <: C)      = [A/^a]_(E) (T |- B <: C)         fv(B + C) ∩ fv(A + E) = Φ
 
 -}
 
-
 mono :: Typ -> Bool
-mono (TForall g)  = False
+mono (TForall g) = False
 mono (TArrow a b) = mono a && mono b
-mono _            = True
+mono _ = True
 
 fv :: Typ -> [Typ]
-fv (TVar i)         = [TVar i]
-fv (TArrow t1 t2)   = fv t1 `union` fv t2
-fv (TForall g)      = fv (g TInt)
-fv _                = []
+fv (TVar i) = [TVar i]
+fv (TArrow t1 t2) = fv t1 `union` fv t2
+fv (TForall g) = fv (g TInt)
+fv _ = []
 
 fvInWork :: Work -> [Typ]
 fvInWork (WVar i) = []
@@ -105,11 +106,13 @@ fvInWork (WExVar j lbs ubs) = nub (concatMap fv lbs) `union` nub (concatMap fv u
 fvInWork (Sub t1 t2) = nub (fv t1) `union` nub (fv t2)
 
 worksToTyps :: [Work] -> [Either Int Int]
-worksToTyps = concatMap (\case
-                          WVar i -> [Left i]
-                          WExVar i _ _ -> [Right i]
-                          _ -> []
-                        )
+worksToTyps =
+  concatMap
+    ( \case
+        WVar i -> [Left i]
+        WExVar i _ _ -> [Right i]
+        _ -> []
+    )
 
 getVarsBeforeTyp :: [Work] -> Typ -> [Typ]
 getVarsBeforeTyp wl (TVar i) = map TVar $ dropWhile (/= i) $ worksToTyps wl
@@ -126,13 +129,15 @@ updateBoundInWL :: Typ -> (BoundTyp, Typ) -> [Work] -> Either String [Work]
 -- match once and no more recursion
 updateBoundInWL var@(TVar (Right i)) bound (WExVar j lbs ubs : ws)
   | i == j =
-      case bound of
-        (LB, typ) -> if var `elem` fVars then Left $  "Error: Cyclic Dependency of " ++ show var ++ " self!"  else Right $ WExVar j (typ:lbs) ubs : ws
-          where fVars = nub $ fv typ
-        (UB, typ) -> if var `elem` fVars then Left $  "Error: Cyclic Dependency of " ++ show var ++ " self!" else Right $ WExVar j lbs (typ:ubs) : ws
-          where fVars = nub $ fv typ
+    case bound of
+      (LB, typ) -> if var `elem` fVars then Left $ "Error: Cyclic Dependency of " ++ show var ++ " self!" else Right $ WExVar j (typ : lbs) ubs : ws
+        where
+          fVars = nub $ fv typ
+      (UB, typ) -> if var `elem` fVars then Left $ "Error: Cyclic Dependency of " ++ show var ++ " self!" else Right $ WExVar j lbs (typ : ubs) : ws
+        where
+          fVars = nub $ fv typ
   | otherwise = updateBoundInWL var bound ws >>= (\ws' -> Right $ WExVar j lbs ubs : ws')
-updateBoundInWL var bound (w:ws) = updateBoundInWL var bound ws >>= (\ws' -> Right $ w : ws')
+updateBoundInWL var bound (w : ws) = updateBoundInWL var bound ws >>= (\ws' -> Right $ w : ws')
 updateBoundInWL var bound [] = error "Bug: Var not found!"
 
 addTypsBefore :: Typ -> [Typ] -> [Work] -> [Work]
@@ -144,7 +149,7 @@ addTypsBefore var@(TVar (Right i)) new_vars (WExVar j lbs ubs : ws)
     typToWork (TVar (Left i)) = WVar i
     typToWork (TVar (Right i)) = WExVar i [] []
     typToWork _ = error "Bug: Incorrect typeToWork call"
-addTypsBefore var new_vars (w:ws) = w : addTypsBefore var new_vars ws
+addTypsBefore var new_vars (w : ws) = w : addTypsBefore var new_vars ws
 addTypsBefore var new_vars [] = error ("Bug: Typ " ++ show var ++ "is not in the worklist")
 
 -- https://stackoverflow.com/questions/27726739/implementing-an-efficient-sliding-window-algorithm-in-haskell
@@ -157,84 +162,91 @@ generateOneSideConstraints bounds = map (\ts -> Sub (head ts) (last ts)) (window
 -- targetTyp, boundTyp, worklist
 carryBackInWL :: Typ -> Typ -> [Work] -> Either String [Work]
 carryBackInWL targetTyp@(TVar (Right i)) boundTyp wl =
-    carryBackInWLHelper wl [] fVars
-    where
-      carryBackInWLHelper :: [Work] -> [Work] -> [Typ] -> Either String [Work]
-      carryBackInWLHelper (wexvar@(WExVar j lbs ubs):wl') toCarryBack fvs
-        | i == j = Right $ wexvar:(reverse toCarryBack++wl')
-        | otherwise = if
-          | (TVar (Right j) `notElem` fvs) ->
-            carryBackInWLHelper wl' toCarryBack fvs >>= (\wl'' -> Right $ wexvar:wl'')
-          | (TVar (Right j) `elem` fvs) && (TVar (Right i) `notElem` fvInWork wexvar) ->
-            carryBackInWLHelper wl' (wexvar:toCarryBack) (fvInWork wexvar `union` fvs)
-          | otherwise -> Left $ "Error: Cyclic Dependency of " ++ show targetTyp ++ " and " ++ show (TVar (Right j))
-      carryBackInWLHelper (wvar@(WVar j):wl') toCarryBack fvs
-        | TVar (Left j) `elem` fvs = Left $ "Error: Cyclic Dependency of " ++ show targetTyp ++ " and " ++ show (TVar (Left j))
-        | otherwise = carryBackInWLHelper wl' toCarryBack fvs >>= (\wl'' -> Right $ wvar:wl'')
-      carryBackInWLHelper (wsub@(Sub t1 t2):wl') toCarryBack fvs =
-        carryBackInWLHelper wl' toCarryBack fvs >>= (\wl'' -> Right $ wsub:wl'')
-      carryBackInWLHelper [] _ _ = Left "Bug: Impossible in carryBackInWL"
-      fVars :: [Typ]
-      fVars = nub $ fv boundTyp
+  carryBackInWLHelper wl [] fVars
+  where
+    carryBackInWLHelper :: [Work] -> [Work] -> [Typ] -> Either String [Work]
+    carryBackInWLHelper (wexvar@(WExVar j lbs ubs) : wl') toCarryBack fvs
+      | i == j = Right $ wexvar : (reverse toCarryBack ++ wl')
+      | otherwise =
+        if
+            | (TVar (Right j) `notElem` fvs) ->
+              carryBackInWLHelper wl' toCarryBack fvs >>= (\wl'' -> Right $ wexvar : wl'')
+            | (TVar (Right j) `elem` fvs) && (TVar (Right i) `notElem` fvInWork wexvar) ->
+              carryBackInWLHelper wl' (wexvar : toCarryBack) (fvInWork wexvar `union` fvs)
+            | otherwise -> Left $ "Error: Cyclic Dependency of " ++ show targetTyp ++ " and " ++ show (TVar (Right j))
+    carryBackInWLHelper (wvar@(WVar j) : wl') toCarryBack fvs
+      | TVar (Left j) `elem` fvs = Left $ "Error: Cyclic Dependency of " ++ show targetTyp ++ " and " ++ show (TVar (Left j))
+      | otherwise = carryBackInWLHelper wl' toCarryBack fvs >>= (\wl'' -> Right $ wvar : wl'')
+    carryBackInWLHelper (wsub@(Sub t1 t2) : wl') toCarryBack fvs =
+      carryBackInWLHelper wl' toCarryBack fvs >>= (\wl'' -> Right $ wsub : wl'')
+    carryBackInWLHelper [] _ _ = Left "Bug: Impossible in carryBackInWL"
+    fVars :: [Typ]
+    fVars = nub $ fv boundTyp
 carryBackInWL _ _ _ = error "Bug: Wrong targetTyp in carryBackInWL"
 
-
 step :: Int -> [Work] -> (Int, Either String [Work], String)
-step n (WVar i : ws)                            = (n, Right ws, "Garbage Collection")     -- 01 
-step n (WExVar i lbs ubs : ws)  
+step n (WVar i : ws) = (n, Right ws, "Garbage Collection") -- 01
+step n (WExVar i lbs ubs : ws)
   | null lbs && null ubs = (n, Right ws, "SUnfoldBoundsEmptyLU")
-  | null lbs = (n, Right $ [Sub (head ubs) uTyp | uTyp <- tail ubs] ++ ws, "SUnfoldBoundsEmptyL")                
-  | null ubs = (n, Right $ [Sub (head lbs) uTyp | uTyp <- tail lbs] ++ ws, "SUnfoldBoundsEmptyU")                 
+  | null lbs = (n, Right $ [Sub (head ubs) uTyp | uTyp <- tail ubs] ++ ws, "SUnfoldBoundsEmptyL")
+  | null ubs = (n, Right $ [Sub (head lbs) uTyp | uTyp <- tail lbs] ++ ws, "SUnfoldBoundsEmptyU")
   | otherwise = (n, Right $ [Sub lTyp uTyp | lTyp <- lbs, uTyp <- ubs] ++ ws, "SUnfoldBounds")
-step n (Sub TInt TInt : ws)                     = (n, Right ws, "SInt")                   -- 03
-step n (Sub TBool TBool : ws)                   = (n, Right ws, "SBool")                  -- 03
-
-step n (Sub (TVar i) (TVar j) : ws)| i == j     = (n, Right ws, "SUVar")                  -- 04 + 05
-step n (Sub (TArrow a b) (TArrow c d) : ws)     =                                         -- 06
-  (n, Right $  Sub b d : Sub c a : ws, "SArrow")
-
-step n (Sub a (TForall g) : ws)                 =                                         -- 08
-  (n+1, Right $ Sub a (g (TVar (Left n))) : WVar n : ws, "SForallR")
-step n (Sub (TForall g) b : ws)                 =                                         -- 07
-  (n+1, Right $  Sub (g (TVar (Right n))) b : WExVar n [] [] : ws, "SForallL")
-
-step n (Sub (TVar (Right i)) (TArrow a b) : ws)                                           -- 09
-   | not $ mono (TArrow a b)                    =
-    (n+2, updateBoundInWL (TVar (Right i)) (UB, a1_a2) (addTypsBefore (TVar (Right i)) [a1, a2] ws) >>=
-      (\wl' -> Right $ Sub (TArrow a1 a2) (TArrow a b):wl'), "SplitL")
-                where
-                  a1 = TVar (Right n)
-                  a2 = TVar $ Right (n + 1)
-                  a1_a2 = TArrow a1 a2
-
-step n (Sub (TArrow a b) (TVar (Right i)) : ws)                                           -- 10
-  | not $ mono (TArrow a b)                     =
-    (n+2, updateBoundInWL (TVar (Right i)) (LB, a1_a2) (addTypsBefore (TVar (Right i)) [a1, a2] ws) >>= 
-      (\wl' -> Right $ Sub (TArrow a b) (TArrow a1 a2) : wl')  , "SplitR")
-                where
-                  a1 = TVar $ Right n
-                  a2 = TVar $ Right (n + 1)
-                  a1_a2 = TArrow a1 a2
-
-step n (Sub (TVar (Right i)) (TVar (Right j)) : ws)                                       -- 15 & 16
-  | prec ws (TVar (Right i)) (TVar (Right j))   =
+step n (Sub TInt TInt : ws) = (n, Right ws, "SInt") -- 03
+step n (Sub TBool TBool : ws) = (n, Right ws, "SBool") -- 03
+step n (Sub (TVar i) (TVar j) : ws) | i == j = (n, Right ws, "SUVar") -- 04 + 05
+step n (Sub (TArrow a b) (TArrow c d) : ws) =
+  -- 06
+  (n, Right $ Sub b d : Sub c a : ws, "SArrow")
+step n (Sub a (TForall g) : ws) =
+  -- 08
+  (n + 1, Right $ Sub a (g (TVar (Left n))) : WVar n : ws, "SForallR")
+step n (Sub (TForall g) b : ws) =
+  -- 07
+  (n + 1, Right $ Sub (g (TVar (Right n))) b : WExVar n [] [] : ws, "SForallL")
+step n (Sub (TVar (Right i)) (TArrow a b) : ws) -- 09
+  | not $ mono (TArrow a b) =
+    ( n + 2,
+      updateBoundInWL (TVar (Right i)) (UB, a1_a2) (addTypsBefore (TVar (Right i)) [a1, a2] ws)
+        >>= (\wl' -> Right $ Sub (TArrow a1 a2) (TArrow a b) : wl'),
+      "SplitL"
+    )
+  where
+    a1 = TVar (Right n)
+    a2 = TVar $ Right (n + 1)
+    a1_a2 = TArrow a1 a2
+step n (Sub (TArrow a b) (TVar (Right i)) : ws) -- 10
+  | not $ mono (TArrow a b) =
+    ( n + 2,
+      updateBoundInWL (TVar (Right i)) (LB, a1_a2) (addTypsBefore (TVar (Right i)) [a1, a2] ws)
+        >>= (\wl' -> Right $ Sub (TArrow a b) (TArrow a1 a2) : wl'),
+      "SplitR"
+    )
+  where
+    a1 = TVar $ Right n
+    a2 = TVar $ Right (n + 1)
+    a1_a2 = TArrow a1 a2
+step n (Sub (TVar (Right i)) (TVar (Right j)) : ws) -- 15 & 16
+  | prec ws (TVar (Right i)) (TVar (Right j)) =
     (n, updateBoundInWL (TVar (Right j)) (LB, TVar (Right i)) ws, "SolveLExtVar")
-  | prec ws (TVar (Right j)) (TVar (Right i))   =
+  | prec ws (TVar (Right j)) (TVar (Right i)) =
     (n, updateBoundInWL (TVar (Right i)) (UB, TVar (Right j)) ws, "SolveRExtVar")
-
-step n (Sub (TVar (Right i)) t : ws)                                        -- 11
-  | mono t                                      =
-    (n, carryBackInWL (TVar (Right i)) t ws >>= 
-      updateBoundInWL (TVar (Right i)) (UB, t), "Solve mono R")
-  | otherwise =  error $ "Bug: Incorrect " ++ show t ++ " !"
-step n (Sub t (TVar (Right i))  : ws)                                       -- 12
-  | mono t                                      =
-    (n, carryBackInWL (TVar (Right i)) t ws >>= 
-      updateBoundInWL (TVar (Right i)) (LB, t), "Solve mono L")
+step n (Sub (TVar (Right i)) t : ws) -- 11
+  | mono t =
+    ( n,
+      carryBackInWL (TVar (Right i)) t ws
+        >>= updateBoundInWL (TVar (Right i)) (UB, t),
+      "Solve mono R"
+    )
   | otherwise = error $ "Bug: Incorrect " ++ show t ++ " !"
-
-step n _                                        = (n, Left "No matched pattern", "None")
-
+step n (Sub t (TVar (Right i)) : ws) -- 12
+  | mono t =
+    ( n,
+      carryBackInWL (TVar (Right i)) t ws
+        >>= updateBoundInWL (TVar (Right i)) (LB, t),
+      "Solve mono L"
+    )
+  | otherwise = error $ "Bug: Incorrect " ++ show t ++ " !"
+step n _ = (n, Left "No matched pattern", "None")
 
 checkAndShow :: Int -> [Work] -> String
 checkAndShow n [] = "Success!"
@@ -242,22 +254,20 @@ checkAndShow n ws =
   case ws' of
     Left e -> "   " ++ show (reverse ws) ++ "\n-->{ Rule: " ++ s1 ++ replicate (20 - length s1) ' ' ++ "Size: " ++ show (size ws) ++ " }\n" ++ e
     Right wl -> s2
-      where s2 = "   " ++ show (reverse ws) ++ "\n-->{ Rule: " ++ s1 ++ replicate (20 - length s1) ' ' ++ "Size: " ++ show (size ws) ++ " }\n" ++ checkAndShow m wl
+      where
+        s2 = "   " ++ show (reverse ws) ++ "\n-->{ Rule: " ++ s1 ++ replicate (20 - length s1) ' ' ++ "Size: " ++ show (size ws) ++ " }\n" ++ checkAndShow m wl
   where
     (m, ws', s1) = step n ws
-
 
 check :: Int -> [Work] -> String
 check n [] = "Success!"
 check n wl =
   let (n', res, s1) = step n wl
-  in
-    case res of
-      Left e -> "Failure!"
-      Right wl' -> check n' wl'
+   in case res of
+        Left e -> "Failure!"
+        Right wl' -> check n' wl'
 
-
-size :: [Work] -> (Int,Int)
+size :: [Work] -> (Int, Int)
 size ws = (measure1 ws, sizeWL ws)
 
 -- Measure 1
@@ -266,10 +276,10 @@ measure1 :: [Work] -> Int
 measure1 ws = 3 * splits ws + foralls ws + existentials ws
 
 splits :: [Work] -> Int
-splits []              = 0
-splits (WVar {} : ws)   = splits ws
-splits (WExVar {}:ws) = splits ws
-splits (Sub a b : ws)  = splitsSub a b + splits ws
+splits [] = 0
+splits (WVar {} : ws) = splits ws
+splits (WExVar {} : ws) = splits ws
+splits (Sub a b : ws) = splitsSub a b + splits ws
 
 splitsSub :: Typ -> Typ -> Int
 splitsSub (TVar (Right i)) t1@(TArrow _ _) = splitsTyp t1
@@ -278,31 +288,31 @@ splitsSub (TArrow a b) (TArrow c d) =
   splitsSub c a + splitsSub b d
 splitsSub a (TForall g) = splitsSub a (g (TVar (Left 0)))
 splitsSub (TForall g) a = splitsSub (g (TVar (Right 0))) a
-splitsSub a b           = 0
+splitsSub a b = 0
 
 splitsTyp :: Num a => Typ -> a
 splitsTyp (TArrow a b)
   | not (mono a) && not (mono b) = 1 + splitsTyp a + splitsTyp b
-  | not (mono a)                 = 1 + splitsTyp a
-  | not (mono b)                 = 1 + splitsTyp b
-  | otherwise                    = 0
-splitsTyp (TForall g)            = splitsTyp (g TInt)
-splitsTyp _                      = 0
+  | not (mono a) = 1 + splitsTyp a
+  | not (mono b) = 1 + splitsTyp b
+  | otherwise = 0
+splitsTyp (TForall g) = splitsTyp (g TInt)
+splitsTyp _ = 0
 
 existentials :: Num a => [Work] -> a
-existentials []                 = 0
-existentials (WExVar {} : ws)   = 1 + existentials ws
-existentials (_ : ws)           = existentials ws
+existentials [] = 0
+existentials (WExVar {} : ws) = 1 + existentials ws
+existentials (_ : ws) = existentials ws
 
 foralls :: Num a => [Work] -> a
-foralls []                      = 0
-foralls (Sub a b : ws)          = forallsTyp a + forallsTyp b + foralls ws
-foralls (_ : ws)                = foralls ws
+foralls [] = 0
+foralls (Sub a b : ws) = forallsTyp a + forallsTyp b + foralls ws
+foralls (_ : ws) = foralls ws
 
 forallsTyp :: Num a => Typ -> a
-forallsTyp (TForall g)  = 1 + forallsTyp (g TInt)
+forallsTyp (TForall g) = 1 + forallsTyp (g TInt)
 forallsTyp (TArrow a b) = forallsTyp a + forallsTyp b
-forallsTyp _            = 0
+forallsTyp _ = 0
 
 {-
 
@@ -313,44 +323,54 @@ forallsTyp _            = 0
 -- Measure 2
 
 sizeWL :: [Work] -> Int
-sizeWL []              = 0
-sizeWL (Sub a b : ws)  = sizeSub a b + sizeWL ws
-sizeWL (_ : ws)        = 1 + sizeWL ws
-
+sizeWL [] = 0
+sizeWL (Sub a b : ws) = sizeSub a b + sizeWL ws
+sizeWL (_ : ws) = 1 + sizeWL ws
 
 sizeSub (TArrow a b) (TArrow c d) = 1 + sizeSub c a + sizeSub b d
-sizeSub (TForall g) a             = 2 + sizeSub (g TInt) a
-sizeSub a (TForall g)             = 2 + sizeSub a (g TInt)
-sizeSub _ _                       = 1
+sizeSub (TForall g) a = 2 + sizeSub (g TInt) a
+sizeSub a (TForall g) = 2 + sizeSub a (g TInt)
+sizeSub _ _ = 1
 
-
-
-chkAndShow = putStrLn .  checkAndShow 0
+chkAndShow = putStrLn . checkAndShow 0
 
 chk :: [Work] -> String
 chk = check 0
 
 test1 = chkAndShow [Sub t3 t3]
+
 test2 = chkAndShow [Sub t1 t3]
+
 test3 = chkAndShow [Sub t5 t3]
+
 test4 = chkAndShow [Sub t5 t1]
+
 test5 = chkAndShow [Sub t1 t6]
+
 test6 = chkAndShow [Sub t6 t3]
+
 test7 = chkAndShow [Sub t5 t7]
+
 test8 = chkAndShow [Sub (TForall $ \a -> TArrow a a) (TArrow t5 (TArrow TInt TInt))]
+
 test9 = chkAndShow [Sub ex1 (TArrow TInt ex2), Sub ex2 (TArrow TInt ex1), WExVar 2 [] [], WExVar 1 [] []]
-test10 = chkAndShow [Sub (TForall (\t -> (TArrow t (TForall (\t1 -> TArrow t1 t))))) (TForall (\t -> (TArrow t (TArrow t t)))) ]
-ws1 = [Sub ex1 (TArrow TInt (TArrow ex2 ex3)), Sub ex2 (TArrow TInt ex1),  WExVar 2 [] [],   WExVar 3 [] [], WExVar 1 [] []]
+
+test10 = chkAndShow [Sub (TForall (\t -> (TArrow t (TForall (\t1 -> TArrow t1 t))))) (TForall (\t -> (TArrow t (TArrow t t))))]
+
+ws1 = [Sub ex1 (TArrow TInt (TArrow ex2 ex3)), Sub ex2 (TArrow TInt ex1), WExVar 2 [] [], WExVar 3 [] [], WExVar 1 [] []]
 
 test12 = chkAndShow [Sub t8 t9]
 
 ex0 = TVar (Right 0)
 
-jimmy = putStrLn $ checkAndShow 3 [
-  Sub TInt TInt,
-  Sub ex0 (TArrow TInt TInt),
-  Sub (TArrow ex0 (TArrow ex0 $ TForall $ \a -> a)) ex1,
-  WExVar 0 [] [],
-  WExVar 1 [] [],
-  WExVar 2 [] []
-  ]
+jimmy =
+  putStrLn $
+    checkAndShow
+      3
+      [ Sub TInt TInt,
+        Sub ex0 (TArrow TInt TInt),
+        Sub (TArrow ex0 (TArrow ex0 $ TForall $ \a -> a)) ex1,
+        WExVar 0 [] [],
+        WExVar 1 [] [],
+        WExVar 2 [] []
+      ]
