proof/transfer.v
@@ -1,7 +1,13 @@
+Require Import Coq.Program.Equality.
+Require Import Program.Tactics.
 Require Import Metalib.Metatheory.
 
 Require Import algo.ott.
 Require Import decl.ott.
+Require Import algo.notations.
+Require Import decl.notations.
+Require Import decl.ln_inf_extra.
+Require Import ln_utils.
 
 
 Inductive ss_entry := 
@@ -17,33 +23,39 @@ Bind Scope subst_set_scope with subst_set.
 Notation "s1 ;; s2" := (app s2 s1)
   (at level 58, left associativity) : subst_set_scope.
 
-Notation "s ; x : t" := (cons (pair x (sse_ev t)) s)
-  ( at level 58, x at next level, left associativity) : subst_set_scope.
+Notation "s ; ex : t" := (cons (pair ex (sse_ev t)) s)
+  (at level 58, ex at next level, t at next level, left associativity) : type_scope.
 
 Notation "s ; x" := (cons (pair x sse_tv) s)
-  ( at level 58, left associativity) : subst_set_scope.
+  (at level 58, x at next level, left associativity) : type_scope.
 
 Notation "x : t ∈ s" := (binds x (sse_ev t) s)
-   (at level 58, t at next level, no associativity) : type_scope.
+  (at level 58, t at next level, no associativity) : type_scope.
 
 
-Fixpoint ss_to_ctx (s : subst_set) : ld_context := 
-  match s with 
-  | nil => ld_ctx_nil
-  | (cons (pair x sse_tv) s') => ld_ctx_cons (ss_to_ctx s') x
-  | (cons (pair x (sse_ev t)) s') => ss_to_ctx s'
+Fixpoint fv_ss (θ : subst_set) : atoms :=
+  match θ with
+  | nil => {}
+  | θ' ; ex : t => fv_ss θ' `union` singleton ex
+  | θ' ; x => fv_ss θ' `union` singleton x
   end.
 
+Fixpoint ss_to_ctx (θ : subst_set) : ld_context := 
+  match θ with 
+  | nil => ld_ctx_nil
+  | θ' ; x => ld_ctx_cons (ss_to_ctx θ') x
+  | θ' ; ex : t => ss_to_ctx θ'
+  end.
 
 Inductive wf_ss : subst_set -> Prop :=
   | wf_ss_nil : wf_ss nil
   | wf_ss_tv : forall x θ,
       wf_ss θ -> x `notin` dom θ ->
       wf_ss (θ; x)
-  | wf_ss_ev : forall x t Θ
-    , wf_ss Θ -> x `notin` dom Θ ->
+  | wf_ss_ev : forall ex t Θ
+    , wf_ss Θ -> ex `notin` dom Θ ->
      ld_wf_mtype (ss_to_ctx Θ) t -> 
-     wf_ss (Θ; x : t)
+     wf_ss (Θ; ex : t)
 .
 
 Lemma wf_uniq : forall Θ,
@@ -53,23 +65,23 @@ Proof.
 Qed.
 
 
-Reserved Notation "θ ⊢ t ⇝ t'"
+Reserved Notation "θ ⫦ t ⇝ t'"
   (at level 65, t at next level, no associativity).
 Inductive inst_type : subst_set -> la_type -> ld_type -> Prop := 
-  | inst_t_tvar : forall θ x, wf_ss θ -> θ ⊢ (la_t_tvar_f x) ⇝ (ld_t_var_f x)
-  | inst_t_evar : forall θ x t, wf_ss θ -> x : t ∈ θ -> θ ⊢ (la_t_evar x) ⇝ t
-  | inst_t_int : forall θ, wf_ss θ -> θ ⊢ la_t_int ⇝ ld_t_int
+  | inst_t_tvar : forall θ x, wf_ss θ -> θ ⫦ (la_t_tvar_f x) ⇝ (ld_t_var_f x)
+  | inst_t_evar : forall θ x t, wf_ss θ -> x : t ∈ θ -> θ ⫦ (la_t_evar x) ⇝ t
+  | inst_t_int : forall θ, wf_ss θ -> θ ⫦ la_t_int ⇝ ld_t_int
   | inst_t_arrow : forall θ A' B' A B, 
-      θ ⊢ A' ⇝ A -> θ ⊢ B' ⇝ B ->
-      θ ⊢ (la_t_arrow A' B') ⇝ (ld_t_arrow A B)
+      θ ⫦ A' ⇝ A -> θ ⫦ B' ⇝ B ->
+      θ ⫦ (la_t_arrow A' B') ⇝ (ld_t_arrow A B)
   | inst_t_forall : forall θ L A' A,
       (forall x, x `notin` L -> 
-      θ ⊢ (open_la_type_wrt_la_type A' (la_t_tvar_f x)) ⇝ (open_ld_type_wrt_ld_type A (ld_t_var_f x))) ->
-      θ ⊢ (la_t_forall A') ⇝ (ld_t_forall A)
-where "θ ⊢ t ⇝ t'" := (inst_type θ t t').
+      θ ⫦ (open_la_type_wrt_la_type A' (la_t_tvar_f x)) ⇝ (open_ld_type_wrt_ld_type A (ld_t_var_f x))) ->
+      θ ⫦ (la_t_forall A') ⇝ (ld_t_forall A)
+where "θ ⫦ t ⇝ t'" := (inst_type θ t t').
 
 Lemma inst_t_wf_ss : forall θ t t',
-  θ ⊢ t ⇝ t' -> wf_ss θ.
+  θ ⫦ t ⇝ t' -> wf_ss θ.
 Proof.
   induction 1; pick fresh x'; eauto.
 Qed.
@@ -84,29 +96,148 @@ Inductive inst_ev : subst_set -> var -> la_typelist -> la_typelist -> Prop :=
 .
 
 
-(* Lemma split : theta |- awl --> dwl -| theta1 -> exists theta0,  theta |- awl  *)
-
-Reserved Notation "θ ⊢ Γ ⇝ Γ' ⊣ θ'"
-  (at level 65,Γ at next level, Γ' at next level, no associativity).
+Reserved Notation "θ ⫦ Γᵃ ⇝ Γᵈ ⫣ θ'"
+  (at level 65, Γᵃ at next level, Γᵈ at next level, no associativity).
 Inductive inst_worklist : subst_set -> la_worklist -> ld_worklist -> subst_set -> Prop := 
   | inst_wl_nil : forall θ, 
-      wf_ss θ -> θ ⊢ la_wl_nil ⇝ ld_wl_nil ⊣ θ
-  | inst_wl_sub : forall θ θ' awl dwl t1 t2 t1' t2', 
-      inst_worklist θ awl dwl θ' -> 
-      inst_type θ' t1 t1' -> 
-      inst_type θ' t2 t2' -> 
-      inst_worklist θ (la_wl_cons_w awl (la_w_sub t1 t2)) (ld_wl_cons_w dwl (ld_w_sub t1' t2')) θ'
-  | inst_wl_tv : forall θ θ' x awl dwl, 
-      inst_worklist θ awl dwl θ' -> 
-      inst_worklist θ (la_wl_cons_tv awl x) (ld_wl_cons_tv dwl x) θ'
-  | inst_wl_ev : forall θ θ' t lbs ex ubs awl dwl, 
-      inst_worklist θ awl dwl θ' -> 
-      ld_mono_type t -> 
+      wf_ss θ -> 
+      θ ⫦ la_wl_nil ⇝ ld_wl_nil ⫣ θ
+  | inst_wl_sub : forall θ θ' Γᵃ t1ᵃ t2ᵃ Γᵈ t1ᵈ t2ᵈ, 
+      θ ⫦ Γᵃ ⇝ Γᵈ ⫣ θ' -> 
+      θ' ⫦ t1ᵃ ⇝ t1ᵈ -> 
+      θ' ⫦ t2ᵃ ⇝ t2ᵈ -> 
+      θ ⫦ (la_wl_cons_w Γᵃ (la_w_sub t1ᵃ t2ᵃ)) ⇝ (ld_wl_cons_w Γᵈ (ld_w_sub t1ᵈ t2ᵈ)) ⫣ θ'
+  | inst_wl_tv : forall θ θ' x Γᵃ Γᵈ, 
+      θ ⫦ Γᵃ ⇝ Γᵈ ⫣ θ' -> 
+      θ ⫦ (la_wl_cons_tv Γᵃ x) ⇝ (ld_wl_cons_tv Γᵈ x) ⫣ θ'
+  | inst_wl_ev : forall θ θ' tᵈ lbs ex ubs Γᵃ Γᵈ, 
+      θ ⫦ Γᵃ ⇝ Γᵈ ⫣ θ' -> 
+      ld_mono_type tᵈ -> 
       ex `notin` dom θ' -> 
-      inst_ev (θ' ; ex : t) ex lbs ubs -> 
-      inst_worklist θ (la_wl_cons_ev awl lbs ex ubs) dwl (θ' ; ex : t)
-where "θ ⊢ Γ ⇝ Γ' ⊣ θ'" := (inst_worklist θ Γ Γ' θ').
+      inst_ev (θ' ; ex : tᵈ) ex lbs ubs -> 
+      θ ⫦ (la_wl_cons_ev Γᵃ lbs ex ubs) ⇝ Γᵈ ⫣ (θ' ; ex : tᵈ)
+where "θ ⫦ Γᵃ ⇝ Γᵈ ⫣ θ'" := (inst_worklist θ Γᵃ Γᵈ θ').
 
 
-Definition transfer (Γ : la_worklist) (Γ' : ld_worklist) : Prop :=
-  exists θ', inst_worklist nil Γ Γ' θ'.
+Lemma notin_ss_notin_inst : forall x ex Θ A,
+    ex : A ∈ Θ → x `notin` fv_ss Θ → x `notin` fv_ld_type A.
+Proof.
+  induction Θ; intros.
+  - inversion H.
+  - destruct a. destruct H.
+    + inversion H; subst; simpl in *; auto. admit.
+    + simpl in H0; eauto.
+Admitted.
+
+
+Lemma ld_t_forall_eq_inj: forall A₁ A₂,
+  A₁ = A₂ -> ld_t_forall A₁ = ld_t_forall A₂.
+Proof.
+  intros.
+  induction H.
+  auto.
+Qed.
+
+(* Alvin *)
+Lemma inst_A_wf_A: forall θ Aᵃ Aᵈ, 
+  θ ⫦ Aᵃ ⇝ Aᵈ -> ss_to_ctx θ ⊢ Aᵈ.
+Proof.
+  intros.
+  dependent induction H.
+Admitted.
+
+Lemma inst_A_det : forall θ Aᵃ A₁ᵈ,
+  uniq θ -> θ ⫦ Aᵃ ⇝ A₁ᵈ -> forall A₂ᵈ, θ ⫦ Aᵃ ⇝ A₂ᵈ -> A₁ᵈ = A₂ᵈ.
+Proof.
+  induction 2; (intros e₂ᵈ H2; dependent destruction H2; auto). 
+  - specialize (binds_unique _ _ _ _ _ H1 H3).
+    intros. specialize (H4 H). inversion H4. auto.
+  - specialize (IHinst_type1 H _ H2_).
+    specialize (IHinst_type2 H _ H2_0).
+    subst. auto.
+  - inst_cofinites_by (L `union` L0 `union` (fv_ld_type A) `union` (fv_ld_type A0)).  
+    assert (A = A0).
+    + eapply open_ld_type_wrt_ld_type_inj with (x1:=x); auto.
+    + subst. auto. 
+Qed.
+
+Locate "[".
+
+(* Ltac rewrite_subst_open_var :=
+  repeat
+    match goal with 
+      | _ : _ |-  context [ ([?e /ᵃ ?x] ?A) ^`′ ?x' ] => 
+        replace (` x') with ([e /ᵃ x] ^`′ x') by (apply subst_la_type_fresh_eq; auto)
+    end; repeat rewrite <- subst_la_type_open_la_type_wrt_la_type by auto. *)
+Lemma inst_e_rename : forall θ Aᵃ Aᵈ x x'
+  , θ ⫦ Aᵃ ⇝ Aᵈ 
+  -> x `notin` dom θ
+  -> θ ⫦ [`′ x' /ᵃ x] Aᵃ ⇝ [` x' /ᵈ x] Aᵈ.
+Proof.
+  intros. induction H; simpl; auto.
+  - unfold eq_dec. destruct (EqDec_eq_of_X x0 x). 
+Admitted.
+
+Lemma inst_e_rev_subst' : forall tᵃ tᵈ x θ Aᵃ
+  , lc_la_type Aᵃ
+  -> x `notin` (fx_la_type tᵃ `union` fv_ss θ) 
+  -> θ ⫦ tᵃ ⇝ tᵈ
+  -> forall A'ᵈ
+  , θ ⫦ subst_la_type tᵃ x Aᵃ ⇝ A'ᵈ
+  -> exists Aᵈ, [tᵈ /ᵈ x] Aᵈ = A'ᵈ /\ θ ⫦ Aᵃ ⇝ Aᵈ.
+Proof.
+  intros * Hlc Hfv Hinstt.
+  induction Hlc; intros * HinstA; simpl in *.
+  - inversion HinstA. exists ld_t_int. simpl. split.
+    + auto.
+    + constructor. auto.
+  - dependent destruction HinstA.
+    inst_cofinites_by (L `union` singleton x `union` fv_ld_type tᵈ `union`  fv_ld_type A). 
+    replace (`′ x0) with ([tᵃ /ᵃ x] `′ x0) in H1 by (apply subst_la_type_fresh_eq; auto).
+    rewrite <- subst_la_type_open_la_type_wrt_la_type in H1.
+    specialize (H0 _ _ H1).
+    destruct H0 as [A'ᵈ HinstA'ᵈ].
+    exists (ld_t_forall (close_ld_type_wrt_ld_type x0 A'ᵈ)). simpl.
+    rewrite subst_ld_type_close_ld_type_wrt_ld_type. 
+    + split.
+      * f_equal. destruct_conjs. apply ld_type_open_r_close_l; auto. 
+      * eapply inst_t_forall with (L:=L); intros.
+
+    + admit. (* lc *)
+    + auto.
+    + auto.
+    + admit. (* lc *)
+  - dependent destruction HinstA.
+    specialize (IHHlc1 _ HinstA1). destruct IHHlc1 as [t₁ᵈ HinstA1inv].
+    specialize (IHHlc2 _ HinstA2). destruct IHHlc2 as [t₂ᵈ HinstA2inv].
+    exists (ld_t_arrow t₁ᵈ t₂ᵈ). destruct_conjs. split.
+    + simpl. subst. auto.
+    + constructor; auto.
+  - exists (ld_t_var_f x5).
+    destruct (x5 == x).  
+    + subst. simpl. destruct (x==x).
+      * split.
+        -- assert (uniq θ) as Huniq by (apply wf_uniq; eapply inst_t_wf_ss; eauto).
+           specialize (inst_A_det _ _ _ Huniq Hinstt). intros.
+           specialize (H _ HinstA). auto.
+        -- constructor. eapply inst_t_wf_ss. eauto.
+      * contradiction.
+    + simpl. unfold eq_dec. destruct (EqDec_eq_of_X x5 x).
+      * contradiction.
+      * inversion HinstA; split; auto. constructor. eapply inst_t_wf_ss; eauto.
+  - simpl in *. exists A'ᵈ. split.
+    + admit.
+    + auto.
+Admitted.
+
+
+Lemma inst_e_rev_subst : forall t' t x θ A'
+  , lc_la_type A'
+  -> x `notin` (fx_la_type t') -> θ ⫦ t' ⇝ t
+  -> forall e0
+  , θ ⫦ subst_la_type t' x A' ⇝ e0
+  -> exists A, [t /ᵈ x] A = e0 /\ θ ⫦ A' ⇝ A.
+Proof.
+
+
+Admitted.
