proof/decl/ln_inf_extra.v
@@ -1,0 +1,12 @@
+Require Import decl.ott.
+Require Export decl.notations.
+
+
+Lemma ld_type_open_r_close_l : forall t1 t2 x
+  , x `notin` fv_ld_type t2
+  -> t1 = open_ld_type_wrt_ld_type t2 `x -> close_ld_type_wrt_ld_type x t1 = t2.
+Proof.
+  intros * Fr H.
+  assert (close_ld_type_wrt_ld_type x t1 = close_ld_type_wrt_ld_type x (open_ld_type_wrt_ld_type t2 `x)) by now rewrite H.
+  now rewrite close_ld_type_wrt_ld_type_open_ld_type_wrt_ld_type in H0.
+Qed.
