proof/decl/properties.v
@@ -29,7 +29,7 @@ Tactic Notation "pick" "fresh" ident(x) "and" "apply" constr(H) "for" "weakening
   apply_fresh_base_fixed H gather_for_weakening x.
 
 Lemma subst_same_eq : forall A x,
-  A = [`x /_ x] A.
+  A = [`x /ᵈ x] A.
 Proof.
   intros.
   induction A; auto.
@@ -41,7 +41,7 @@ Qed.
 
 Lemma open_subst_eq : forall A x t, 
   x `notin` fv_ld_type A -> lc_ld_type t  ->
-    A ^^ t = [t /_ x] A ^^ `x.
+    A ^^ t = [t /ᵈ x] A ^^ `x.
 Proof.
   intros.  
   rewrite subst_ld_type_open_ld_type_wrt_ld_type. simpl.
@@ -218,7 +218,7 @@ Qed.
 
 Theorem ld_wf_mtype_subst :
   forall G1 G2 x t t', 
-    ld_mono_type t' -> ld_wf_mtype (G1, x,, G2) t -> G1 ⊢ t' ->  ld_wf_mtype (G1,, G2) ([t' /_ x] t).
+    ld_mono_type t' -> ld_wf_mtype (G1, x,, G2) t -> G1 ⊢ t' ->  ld_wf_mtype (G1,, G2) ([t' /ᵈ x] t).
 Proof.
   intros.
   dependent induction H0.
@@ -239,8 +239,8 @@ Qed.
 Ltac rewrite_subst_open_var :=
   repeat
     match goal with 
-      | _ : _ |-  context [ ([?e /_ ?x] ?A) ^^ ` ?x' ] => 
-        replace (` x') with ([e /_ x] `x') by (apply subst_ld_type_fresh_eq; auto)
+      | _ : _ |-  context [ ([?e /ᵈ ?x] ?A) ^^ ` ?x' ] => 
+        replace (` x') with ([e /ᵈ x] `x') by (apply subst_ld_type_fresh_eq; auto)
     end; repeat rewrite <- subst_ld_type_open_ld_type_wrt_ld_type by auto.
 
 
@@ -254,7 +254,7 @@ Qed.
 Theorem substitution : forall G1 G2 x A B t,
   G1 , x  ,, G2 ⊢ A <: B ->
   G1 ⊢ t -> ld_mono_type t ->
-  G1 ,, G2 ⊢ [t /_ x] A <: [t /_ x] B.
+  G1 ,, G2 ⊢ [t /ᵈ x] A <: [t /ᵈ x] B.
 Proof.
   intros.
   dependent induction H.
@@ -269,15 +269,15 @@ Proof.
   - simpl. constructor.
     replace (G1, x,, G2) with (G1 ,, (ld_ctx_nil, x),, G2) in * by auto. eapply ld_wf_ctx_weakening; eauto.
   - simpl. constructor; eauto.
-  - simpl. eapply ld_sub_foralll with (t:=[t /_ x] t0). 
+  - simpl. eapply ld_sub_foralll with (t:=[t /ᵈ x] t0). 
     + apply ld_wf_mtype_subst; auto.
-    + replace (([t /_ x] A) ^^ ([t /_ x] t0)) with ([t /_ x] A ^^ t0).
+    + replace (([t /ᵈ x] A) ^^ ([t /ᵈ x] t0)) with ([t /ᵈ x] A ^^ t0).
       * apply IHld_sub; auto.
       * rewrite subst_ld_type_open_ld_type_wrt_ld_type; auto. now apply ld_mono_is_ld_lc.
   - simpl. eapply ld_sub_forallr with (L:=L `union` singleton x).
     intros. inst_cofinites_with x0.
     rewrite_subst_open_var.
-    replace  (([t /_ x] B) ^^ ([t /_ x] ` x0)) with ( [t /_ x] B ^^ ` x0).
+    replace  (([t /ᵈ x] B) ^^ ([t /ᵈ x] ` x0)) with ( [t /ᵈ x] B ^^ ` x0).
     + replace (G1,, G2, x0 ) with (G1,, (G2, x0)) by auto. apply H0; auto.
     + rewrite subst_ld_type_open_ld_type_wrt_ld_type. reflexivity. simpl.
       replace (G1,, G2, x0 ) with (G1,, (G2, x0)) by auto. now apply ld_mono_is_ld_lc.
@@ -401,7 +401,7 @@ Qed.
 Theorem sized_var_substitution : forall G1 G2 x x' A B n,
   G1 , x  ,, G2 ⊢ A <: B | n ->
   ⊢ G1, x' ,, G2 ->
-  G1 , x' ,, G2 ⊢ [`x' /_ x] A <: [`x' /_ x] B | n.
+  G1 , x' ,, G2 ⊢ [`x' /ᵈ x] A <: [`x' /ᵈ x] B | n.
 Proof.
   intros.
   dependent induction H.
@@ -415,9 +415,9 @@ Proof.
         replace (G1,x',,G2) with (G1,,(ld_ctx_nil, x'),,G2) by auto. apply ld_in_context_weakenning. auto.
   - simpl. constructor. auto. 
   - simpl. constructor; eauto.
-  - simpl. eapply sls_foralll with (t:=[`x' /_ x] t). 
+  - simpl. eapply sls_foralll with (t:=[`x' /ᵈ x] t). 
     + destruct (x==x'); subst.
-      * replace ([` x' /_ x'] t) with t; auto.
+      * replace ([` x' /ᵈ x'] t) with t; auto.
         now apply subst_same_eq.
       * apply ld_wf_mtype_equiv_ld_wf_type_and_mono in H. destruct H.
         apply ld_wf_mtype_subst.
@@ -433,13 +433,13 @@ Proof.
                simpl. rewrite <- IHG2. auto.
         -- constructor. replace (G1, x') with (G1,x',,ld_ctx_nil) by auto. eapply ld_wf_ctx_weakening; eauto.
            constructor. 
-    + replace (([`x' /_ x] A) ^^ ([`x' /_ x] t)) with ([`x' /_ x] A ^^ t).
+    + replace (([`x' /ᵈ x] A) ^^ ([`x' /ᵈ x] t)) with ([`x' /ᵈ x] A ^^ t).
       * apply IHsized_ld_sub; auto.
       * rewrite subst_ld_type_open_ld_type_wrt_ld_type; auto. 
   - simpl. eapply sls_forallr with (L:=L `union` singleton x `union` ld_ctx_dom ( G1, x',, G2)).
     intros. inst_cofinites_with x0.
     rewrite_subst_open_var.
-    replace  (([`x' /_ x] B) ^^ ([`x' /_ x] ` x0)) with ( [`x' /_ x] B ^^ ` x0).
+    replace  (([`x' /ᵈ x] B) ^^ ([`x' /ᵈ x] ` x0)) with ( [`x' /ᵈ x] B ^^ ` x0).
     + replace (G1, x',, G2, x0 ) with (G1,x',, (G2, x0)) by auto. apply H0; auto.
       simpl. constructor; auto. 
     + rewrite subst_ld_type_open_ld_type_wrt_ld_type. reflexivity. simpl.
@@ -457,7 +457,7 @@ Hint Extern 1 (?x < ?y) => lia : trans.
 
 
 Lemma ld_sub_to_sized_ld_sub : forall G t1 t2,
-  (ld_sub G t1 t2) -> exists n', G ⊢ t1 <: t2 | n'.
+  G ⊢ t1 <: t2 -> exists n', G ⊢ t1 <: t2 | n'.
 Proof with eauto with trans.
   intros. induction H.
   + exists 0. econstructor; eauto.
@@ -470,8 +470,8 @@ Proof with eauto with trans.
   + inst_cofinites_by (L `union` fv_ld_type A `union` fv_ld_type B). destruct H0 as [n].
     exists (S n). eapply sls_forallr with (L:=L `union` (ld_ctx_dom G)). intros.
     replace (G, x0) with (G, x0,,ld_ctx_nil) by auto.
-    replace A with ([`x0 /_ x] A).
-    replace (B ^^ `x0) with ([`x0 /_ x] B ^^ `x).
+    replace A with ([`x0 /ᵈ x] A).
+    replace (B ^^ `x0) with ([`x0 /ᵈ x] B ^^ `x).
     eapply  sized_var_substitution; eauto.
     * simpl. constructor; auto.
       apply ld_sub_wf_ctx in H. dependent destruction H. auto.
@@ -482,8 +482,8 @@ Qed.
 
 Theorem sized_substitution : forall G1 G2 x A B t n,
   G1 , x  ,, G2 ⊢ A <: B | n ->
-  ld_wf_type G1 t -> ld_mono_type t ->
-  exists n', G1 ,, G2 ⊢ [t /_ x] A <: [t /_ x] B | n'.
+  G1 ⊢ t -> ld_mono_type t ->
+  exists n', G1 ,, G2 ⊢ [t /ᵈ x] A <: [t /ᵈ x] B | n'.
 Proof.
   intros.
   apply sized_ld_sub_to_ld_sub in H.
@@ -495,7 +495,7 @@ Qed.
 Theorem generalized_transitivity : forall t_order t_ssize G A B C n1 n2 ,
   type_order B < t_order ->
   n1 + n2 < t_ssize -> 
-  (G ⊢ A <: B | n1) -> (G ⊢ B <: C | n2) -> (ld_sub G A C).
+  (G ⊢ A <: B | n1) -> (G ⊢ B <: C | n2) -> G ⊢ A <: C.
 Proof with eauto with trans.
   induction t_order; induction t_ssize; intros.
   - inversion H. 
@@ -520,8 +520,8 @@ Proof with eauto with trans.
           eapply IHt_order with (B:=B ^^ t) (n1:=n1) (n2:=n0); eauto. simpl in H; eauto.
           rewrite (open_mono_order B t); eauto...
           replace G with (G ,, ld_ctx_nil) by auto.
-          replace (B ^^ t) with ([t /_ x] B ^^ `x).
-          replace A with ([t /_ x] A).
+          replace (B ^^ t) with ([t /ᵈ x] B ^^ `x).
+          replace A with ([t /ᵈ x] A).
           -- auto. 
           -- rewrite subst_ld_type_fresh_eq; auto.
           -- apply eq_sym. eapply open_subst_eq; auto.
@@ -534,8 +534,8 @@ Proof with eauto with trans.
           assert (⊢ G, x0). { constructor. dependent destruction H5;  auto. auto. }
           replace (G, x, x0) with (G ,, (ld_ctx_nil,  x) ,, (ld_ctx_nil, x0)) by auto.
           eapply sized_ld_sub_weakening; simpl.
-          replace A with ([`x0 /_ x] A).
-          replace (B ^^ `x0) with ([`x0 /_ x] B ^^ `x).
+          replace A with ([`x0 /ᵈ x] A).
+          replace (B ^^ `x0) with ([`x0 /ᵈ x] B ^^ `x).
           replace (G, x0) with (G, x0,, ld_ctx_nil) by auto.
           apply sized_var_substitution; auto.
           -- apply eq_sym. eauto... 
@@ -544,7 +544,7 @@ Proof with eauto with trans.
 Qed.
 
 Theorem transitivity : forall G A B C,
-  (ld_sub G A B) -> (ld_sub G B C) -> (ld_sub G A C).
+  G ⊢ A <: B -> G ⊢ B <: C -> G ⊢ A <: C.
 Proof.
   intros.
   apply ld_sub_to_sized_ld_sub in H. destruct H as [n1].
